Simple assembly for arithmetic expressions

typed-assembly/StaticCode.v
@@ -19,22 +19,20 @@ Fixpoint valid_nth A (l : list A) (n : nat) (H : n < length l) : A.
 Defined.
 
 Module Instr.
-  Inductive t (S : Set) (L : S -> Type)
+  Definition t (S : Set) (L : S -> Type)
     (lt : (nat * sigT L) -> (nat * sigT L) -> Prop) (Hwf : well_founded lt)
     (size : nat) : Type :=
-  | op :
-    (forall s ip, {s'_next_ip : S * nat &
+    forall s ip, {s'_next_ip : S * nat &
       let (s', next_ip) := s'_next_ip in
       forall (l : L s), Datatypes.S ip <= size -> (next_ip <= size) * {l' : L s' |
-      lt (next_ip, existT _ _ l') (Datatypes.S ip, existT _ _ l) }}) ->
-      t Hwf size.
+      lt (next_ip, existT _ _ l') (Datatypes.S ip, existT _ _ l) }}.
   
+  (** Simple eval of just one instruction (for tests) *)
   Definition eval (S : Set) (L : S -> Type)
     (lt : (nat * sigT L) -> (nat * sigT L) -> Prop) (Hwf : well_founded lt)
     (size : nat) (i : t Hwf size)
     (ip : nat) (s : S) (l : L s) (Hip_valid : Datatypes.S ip <= size)
     : {next_ip : nat | next_ip <= size} * {s' : S & L s'}.
-    destruct i as [i].
     destruct (i s ip) as ((s', next_ip), fl).
     destruct (fl l Hip_valid) as (Hnext_ip_valid, (l', _)).
     exact (exist _ next_ip Hnext_ip_valid, existT _ s' l').
@@ -65,7 +63,6 @@ Module Program.
         rewrite Hp_valid in Hip_valid.
         apply lt_S_n.
         now apply le_lt_n_Sm.
-      destruct i as [i].
       destruct (i s ip) as ((s', next_ip), fl).
       destruct (fl l Hip_valid) as (Hnext_ip_valid, (l', Hl'_lt_l)).
       exact (eval (next_ip, existT _ _ l') Hl'_lt_l Hnext_ip_valid).
@@ -94,8 +91,8 @@ Module Test1.
       a proof that it is greater or equal to three. *)
   Definition progr : Program.t lt_wf size.
     refine [
-      op lt_wf size (fun n ip => existT _ (n + 1, ip) _);
-      op lt_wf size (fun _ ip => existT _ (12, ip) _)];
+      (fun n ip => existT _ (n + 1, ip) _);
+      (fun _ ip => existT _ (12, ip) _)];
       unfold S, L, lt; intros l Hip_valid;
       (split; [now apply le_Sn_le |]);
       [assert (H : L (n + 1)) | assert (H : 3 <= 12)]; unfold L; auto with arith;
@@ -112,7 +109,8 @@ Module Test1.
   Qed.
   
   Definition first_op : Instr.t lt_wf size.
-    refine (op lt_wf size (fun n ip => existT _ (n + 1, ip) _)).
+    unfold t.
+    refine (fun n ip => existT _ (n + 1, ip) _).
     unfold S, L, lt; intros l Hip_valid.
     split; [now apply le_Sn_le |].
     assert (H : L (n + 1)); unfold L; auto with arith.
@@ -124,7 +122,7 @@ Module Test1.
   
   Definition progr_small : Program.t lt_wf 1.
     refine [
-      op lt_wf 1 (fun n ip => existT _ (n + 1, ip) _)];
+      fun n ip => existT _ (n + 1, ip) _];
       unfold S, L, lt; intros l Hip_valid;
       (split; [now apply le_Sn_le |]);
       [assert (H : L (n + 1))]; unfold L; auto with arith;
@@ -136,3 +134,91 @@ Module Test1.
   
   Compute projT1 (Program.eval progr eq_refl input input_is_valid).
 End Test1.
+
+Module ArithAsm.
+  Require Import ZArith.
+  
+  Local Open Scope Z_scope.
+  
+  Inductive t : Set :=
+  | const (n : Z) | uminus | plus | minus | times.
+  
+  Definition S := list Z.
+  
+  Definition L (s : S) := unit.
+  
+  Definition lt (x y : nat * sigT L) : Prop :=
+    Peano.lt (fst x) (fst y).
+  
+  Lemma lt_wf : well_founded lt.
+    apply well_founded_ltof.
+  Defined.
+  
+  Definition instr_of_state_update size (f : S -> S) : Instr.t lt_wf size.
+    unfold Instr.t.
+    refine (fun s ip =>
+      existT _ (f s, ip) _).
+    intros l Hip_valid.
+    split; [now apply le_Sn_le |].
+    exists tt.
+    unfold lt; auto.
+  Defined.
+  
+  Definition instr_of_unop size (f : Z -> Z) : Instr.t lt_wf size :=
+    instr_of_state_update size (fun s =>
+      match s with
+      | n :: s => f n :: s
+      | _ => s
+      end).
+  
+  Definition instr_of_binop size (f : Z -> Z -> Z) : Instr.t lt_wf size :=
+    instr_of_state_update size (fun s =>
+      match s with
+      | n1 :: n2 :: s => f n1 n2 :: s
+      | _ => s
+      end).
+  
+  Definition to_instr size (i : t) : Instr.t lt_wf size :=
+    match i with
+    | const n => instr_of_state_update size (fun s => n :: s)
+    | uminus => instr_of_unop size (fun n => - n)
+    | plus => instr_of_binop size (fun n1 n2 => n1 + n2)
+    | minus => instr_of_binop size (fun n1 n2 => n1 - n2)
+    | times => instr_of_binop size (fun n1 n2 => n1 * n2)
+    end.
+  
+  Definition compile (p : list t) : Program.t lt_wf (length p) :=
+    List.map (to_instr (length p)) p.
+  
+  Lemma compile_is_valid : forall (p : list t),
+    length (compile p) = length p.
+    intro; apply map_length.
+  Qed.
+  
+  Definition eval (p : list t) : S.
+    refine (projT1 (Program.eval (compile p) _ (length p, existT _ nil tt) _));
+      trivial.
+    now rewrite compile_is_valid.
+  Defined.
+  
+  Module Test.
+    Definition p1 := [const 12].
+    Definition p2 := [uminus; const 12].
+    Definition p3 := [plus; const 12; times; const 5; const 2].
+    
+    Compute eval p1.
+    Compute eval p2.
+    Compute eval p3.
+  End Test.
+End ArithAsm.
+
+
+
+
+
+
+
+
+
+
+
